Adding BLS_WITHDRAWAL_PREFIX byte constant and precondition to updatePubKeyChanges()

src/dafny/beacon/BeaconChainTypes.dfy
@@ -36,6 +36,7 @@ module BeaconChainTypes {
     import opened AttestationsTypes
 
     const MAX_BLOCK_PUBKEY_CHANGES: int := 16;
+    const BLS_WITHDRAWAL_PREFIX: uint8 := 0x00;
 
     datatype PubKeyChange = PubKeyChange ( // PubKeyChange class representation- new in Revoke
         validator_index: ValidatorIndex,
